CrProgramState.v
@@ -54,17 +54,13 @@ Definition new_pmap_from_old {T: Type} (old_pmap : PMap.t T) (f : positive -> T)
    PTree.map (fun x _ => f x) (snd old_pmap) (* Take old tree (snd old_pmap) and map elements from it (x) via function (f) *)
   ).
 
-Section VarlikeMap.
-
-Context {A : Type} `{CrVarLike A}.
-
-Definition lookup_varlike_map {T : Type} (m : PMap.t T) (x : A) : T :=
+Definition lookup_varlike_map {T A : Type} `{CrVarLike A} (m : PMap.t T) (x : A) : T :=
   PMap.get (get_key x) m.
 
-Definition lookup_varlike {T : Type} (f: PSField) (s: ProgramState T) (x : A) : T :=
+Definition lookup_varlike {T A : Type} `{CrVarLike A} (f: PSField) (s: ProgramState T) (x : A) : T :=
   lookup_varlike_map (map_from_ps f s) x.
 
-Definition update_all_varlike {T : Type} (f: PSField) (s: ProgramState T) (fh: A -> T) : ProgramState T :=
+Definition update_all_varlike {T A : Type} `{CrVarLike A} (f: PSField) (s: ProgramState T) (fh: A -> T) : ProgramState T :=
   let new_map := new_pmap_from_old (map_from_ps f s) (fun pos => fh (make_item pos)) in
   match f with
   | PSCtrl =>   {| ctrl_map := new_map;
@@ -78,10 +74,10 @@ Definition update_all_varlike {T : Type} (f: PSField) (s: ProgramState T) (fh: A
                    state_map := new_map |}
   end.
 
-Definition update_varlike_map {T : Type} (m: PMap.t T) (x: A) (v: T) : PMap.t T :=
+Definition update_varlike_map {T A : Type} `{CrVarLike A} (m: PMap.t T) (x: A) (v: T) : PMap.t T :=
   PMap.set (get_key x) v m.
   
-Definition update_varlike {T : Type} (f: PSField) (s: ProgramState T) (x: A) (v: T) : ProgramState T :=
+Definition update_varlike {T A : Type} `{CrVarLike A} (f: PSField) (s: ProgramState T) (x: A) (v: T) : ProgramState T :=
   let new_map := update_varlike_map (map_from_ps f s) x v in
   match f with
   | PSCtrl =>   {| ctrl_map := new_map;
@@ -96,7 +92,7 @@ Definition update_varlike {T : Type} (f: PSField) (s: ProgramState T) (x: A) (v:
   end.
 
 Lemma update_all_varlike_lookup_unchanged:
-  forall {T} (s1 : ProgramState T) (f : PSField),
+  forall {T A} `{CrVarLike A} (s1 : ProgramState T) (f : PSField),
    update_all_varlike f s1 (fun v : A => lookup_varlike_map (map_from_ps f s1) v) = s1.
 Proof.
   intros.
@@ -124,7 +120,7 @@ Proof.
 Qed.
 
 Lemma commute_mapper_lookup_varlike:
-  forall {T1} {T2} ps v (func : T1 -> T2) f,
+  forall {T1 T2 A} `{CrVarLike A} ps v (func : T1 -> T2) f,
   lookup_varlike_map (map_from_ps f (program_state_mapper func func func ps)) v =
   func (lookup_varlike_map (map_from_ps f ps) v).
 Proof.
@@ -134,7 +130,7 @@ Proof.
 Qed.
 
 Lemma commute_mapper_update_varlike:
-  forall {T1} {T2} ps x v (func : T1 -> T2) f,
+  forall {T1 T2 A} `{CrVarLike A} ps x v (func : T1 -> T2) f,
   program_state_mapper func func func (update_varlike f ps x v) =
   update_varlike f (program_state_mapper func func func ps) x (func v).
 Proof.
@@ -163,7 +159,7 @@ Proof.
 Qed.
 
 Lemma lookup_f1_unchanged_by_update_all_f2:
-  forall {T} fs (s1 : ProgramState T) (h : A) f1 f2,
+  forall {T A} `{CrVarLike A} fs (s1 : ProgramState T) (h : A) f1 f2,
   f1 <> f2 ->
     lookup_varlike_map (map_from_ps f1 s1) h =
     lookup_varlike_map (map_from_ps f1 (update_all_varlike f2 s1 fs)) h.
@@ -174,36 +170,54 @@ Proof.
   try congruence.
 Qed.
 
-Definition is_varlike_in_ps {T} (f : PSField) (s1 : ProgramState T) (v : A) :=
+Definition is_varlike_in_ps {T A} `{CrVarLike A} (f : PSField) (s1 : ProgramState T) (v : A) :=
   PTree.get (get_key v) (snd (map_from_ps f s1)).
 
-(* Lemma lookup_varlike_after_update_all_varlike:
-  forall {T} (s1 : ProgramState T) (h : A) (fh : A -> T) (f : PSField),
-    is_varlike_in_ps f s1 h <> None ->
-    lookup_varlike_map (map_from_ps f (update_all_varlike f s1 fh)) h = fh h.
+Lemma lookup_varlike_after_update_all_varlike:
+  forall {T A} `{CrVarLike A} (s1 : ProgramState T) (v : A) (fv : A -> T) field,
+    is_varlike_in_ps field s1 v <> None ->
+    lookup_varlike_map (map_from_ps field (update_all_varlike field s1 fv)) v = fv v.
 Proof.
   intros.
   unfold lookup_varlike_map.
   unfold update_all_varlike.
-  destruct f;
+  destruct field;
   simpl;
   unfold lookup_varlike_map;
   unfold new_pmap_from_old;
-  simpl.
-  - unfold is_varlike_in_ps in H0.
-    destruct (ctrl_map s1) as [default ctrl].
-    simpl.
-    f_equal.
-    unfold PMap.get.
-    simpl.
-    rewrite PTree.gmap.
-    unfold Coqlib.option_map.
-    rewrite inverses.
-    destruct (snd (map_from_ps PSCtrl s1)) ! (get_key h).
-    destruct (ctrl ! (get_key h)) eqn:des; auto.
-Admitted. *)
+  simpl;
+  unfold is_varlike_in_ps in H0; simpl in H0;
+  try destruct (map_from_ps PSCtrl s1) as [default ctrl];
+  try destruct (map_from_ps PSHeader s1) as [default header];
+  try destruct (map_from_ps PSState s1) as [default state];
+  unfold PMap.get;
+  simpl;
+  rewrite PTree.gmap;
+  unfold Coqlib.option_map;
+  rewrite inverses;
+  simpl;
+  simpl in H.
+  - destruct (snd (ctrl_map s1)) ! (get_key v) eqn:des. auto. congruence.
+  - destruct (snd (header_map s1)) ! (get_key v) eqn:des. try auto. congruence.
+  - destruct (snd (state_map s1)) ! (get_key v) eqn:des. try auto. congruence.
+Qed.
 
-End VarlikeMap.
+Lemma commute_varlike_updates:
+  forall {T A A'}
+    `{CrVarLike A}
+    `{CrVarLike A'}
+    (s1 : ProgramState T)
+    (f f' : PSField)
+    (fv : A -> T) (fv' : A' -> T),
+  f <> f' ->
+    update_all_varlike f (update_all_varlike f' s1 fv') fv =
+    update_all_varlike f' (update_all_varlike f s1 fv) fv'.
+Proof.
+  intros.
+  destruct f, f';
+  try congruence;
+  try unfold update_all_varlike; f_equal.
+Qed.
 
 (* TODO: lookup_hdr/state_map could be rolled into lookup_hdr/state. *)
 (* TODO: It is used in a proof with a giant remember expression. *)
@@ -266,62 +280,8 @@ Qed.
 Definition is_header_in_ps {T} (s1 : ProgramState T) (h : Header) :=
   PTree.get (match h with | HeaderCtr id => id end) (snd (header_map s1)).
 
-Lemma lookup_hdr_after_update_all_hdrs:
-  forall {T} (s1 : ProgramState T) (h : Header) (fh : Header -> T),
-    is_header_in_ps s1 h <> None ->
-    lookup_varlike_map (map_from_ps PSHeader (update_all_varlike PSHeader s1 fh)) h = fh h.
-Proof.
-  intros.
-  unfold lookup_varlike_map.
-  unfold update_all_varlike.
-  simpl.
-  unfold lookup_varlike_map.
-  unfold new_pmap_from_old.
-  simpl.
-  unfold is_header_in_ps in H.
-  destruct (header_map s1) as [default hdr].
-  simpl.
-  f_equal.
-  unfold PMap.get.
-  simpl.
-  rewrite PTree.gmap.
-  unfold Coqlib.option_map.
-  destruct h.
-  simpl.
-  simpl in H.
-  destruct (hdr ! uid) eqn:des; auto.
-  congruence.
-Qed.
-
 Definition is_state_var_in_ps {T} (s1 : ProgramState T) (sv : State) :=
   PTree.get (match sv with | StateCtr id => id end) (snd (state_map s1)).
-
-Lemma lookup_state_after_update_all_states:
-  forall {T} (s1 : ProgramState T) (sv : State) (fs : State -> T),
-    is_state_var_in_ps s1 sv <> None ->
-    lookup_varlike_map (map_from_ps PSState (update_all_varlike PSState s1 fs)) sv = fs sv.
-Proof.
-  intros.
-  unfold lookup_varlike_map.
-  unfold update_all_varlike.
-  simpl.
-  unfold lookup_varlike_map.
-  unfold new_pmap_from_old.
-  simpl.
-  unfold is_state_var_in_ps in H.
-  destruct (state_map s1) as [default sv_map].
-  simpl.
-  f_equal.
-  unfold PMap.get.
-  simpl.
-  rewrite PTree.gmap.
-  unfold Coqlib.option_map.
-  destruct sv.
-  simpl.
-  simpl in H.
-  destruct (sv_map ! uid) eqn:des; auto.
-  congruence.
-Qed.
 
 Lemma commute_state_hdr_updates:
   forall {T} (s1 : ProgramState T) (fh : Header -> T) (fs : State -> T),
