HelperLemmas.v
@@ -38,6 +38,19 @@ Proof.
   reflexivity.
 Qed.
 
+Lemma commute_lookup_eval_ctrl:
+  forall (s : SymbolicState) (f : SmtValuation)
+        hc,
+    lookup_varlike_map (map_from_ps PSCtrl (eval_sym_state s f)) hc =
+    eval_smt_arith (lookup_varlike_map (map_from_ps PSCtrl s) hc) f.
+Proof.
+  intros s f hc.
+  destruct hc.
+  unfold eval_sym_state.
+  rewrite commute_mapper_lookup_varlike.
+  reflexivity.
+Qed.
+
 Lemma commute_lookup_eval:
   forall (s : SymbolicState) (f : SmtValuation)
         arg,
