PMapHelperLemmas.v
@@ -31,11 +31,11 @@ Proof.
 Qed.
 
 (* Same as the above lemma for hdr and state *)
-Transparent lookup_hdr.
+Transparent lookup_varlike.
 Lemma commute_lookup_eval_hdr:
   forall h f s,
-  lookup_hdr (eval_sym_state s f) h =
-  eval_smt_arith (lookup_hdr s h) f.
+  lookup_varlike PSHeader (eval_sym_state s f) h =
+  eval_smt_arith (lookup_varlike PSHeader s h) f.
 Proof.
   intros.
   apply PMap.gmap.
